src/Test.hs
@@ -1,0 +1,228 @@
+{-# LANGUAGE LambdaCase #-}
+{-# LANGUAGE FlexibleContexts #-}
+module Hoare where
+
+import           Control.Monad.State
+import           Control.Monad.Writer
+import qualified Data.Set as S
+import           Data.Set (Set)
+import qualified Data.Map as M
+import           Data.Map (Map)
+
+import Debug.Trace
+
+type Var = String
+
+data Expr
+  = Add Expr Expr
+  | Mul Expr Expr
+  | Sub Expr Expr
+  | Div Expr Expr
+  | Lit Integer
+  | V Var
+  deriving (Show, Read, Eq, Ord)
+
+evocab :: Expr -> Set Var
+evocab = \case
+  Add e1 e2 -> evocab e1 `S.union` evocab e2
+  Mul e1 e2 -> evocab e1 `S.union` evocab e2
+  Sub e1 e2 -> evocab e1 `S.union` evocab e2
+  Div e1 e2 -> evocab e1 `S.union` evocab e2
+  Lit _ -> S.empty
+  V v -> S.singleton v
+
+esubst :: Var -> Expr -> Expr -> Expr
+esubst v e = \case
+  Add e1 e2 -> Add (esubst v e e1) (esubst v e e2)
+  Mul e1 e2 -> Mul (esubst v e e1) (esubst v e e2)
+  Sub e1 e2 -> Sub (esubst v e e1) (esubst v e e2)
+  Div e1 e2 -> Div (esubst v e e1) (esubst v e e2)
+  Lit i -> Lit i
+  V v' -> if v == v' then e else V v'
+
+data Prop
+  = PTrue
+  | PFalse
+  | PImpl Prop Prop
+  | PAnd Prop Prop
+  | PNot Prop
+  | PEql Expr Expr
+  | PLt Expr Expr
+  | PRel Var [Expr]
+  | PForall Var Prop
+  deriving (Show, Read, Eq, Ord)
+
+pvocab :: Prop -> Set Var
+pvocab = \case
+  PTrue -> S.empty
+  PFalse -> S.empty
+  PImpl p1 p2 -> pvocab p1 `S.union` pvocab p2
+  PAnd p1 p2 -> pvocab p1 `S.union` pvocab p2
+  PNot p -> pvocab p
+  PEql e1 e2 -> evocab e1 `S.union` evocab e2
+  PLt e1 e2 -> evocab e1 `S.union` evocab e2
+  PRel v es -> S.unions (map evocab es)
+
+psubst :: Var -> Expr -> Prop -> Prop
+psubst v e = \case
+  PTrue -> PTrue
+  PFalse -> PFalse
+  PImpl p1 p2 -> PImpl (psubst v e p1) (psubst v e p2)
+  PAnd p1 p2 -> PAnd (psubst v e p1) (psubst v e p2)
+  PNot p -> PNot (psubst v e p)
+  PEql e1 e2 -> PEql (esubst v e e1) (esubst v e e2)
+  PLt e1 e2 -> PLt (esubst v e e1) (esubst v e e2)
+  PRel n es -> PRel n (map (esubst v e) es)
+
+data Com
+  = Skip
+  | Assign Var Expr
+  | If Prop Com Com
+  | Seq Com Com
+  | While Prop Com
+  | Assert Prop
+  | Prod Com Com
+  | Fail
+  deriving (Show, Read, Eq, Ord)
+
+cvocab :: Com -> Set Var
+cvocab = \case
+  Skip -> S.empty
+  Assign v e -> S.insert v (evocab e)
+  If p c1 c2 -> S.unions [pvocab p, cvocab c1, cvocab c2]
+  Seq c1 c2 -> cvocab c1 `S.union` cvocab c2
+  Prod c1 c2 -> cvocab c1 `S.union` cvocab c2
+  While p c -> pvocab p `S.union` cvocab c
+  Fail -> S.empty
+
+data HoareState = HoareState
+  { counter :: Integer
+  , relations :: Map Com Prop
+  } deriving (Show, Read, Eq, Ord)
+
+emptyHoareState :: HoareState
+emptyHoareState = HoareState
+  { counter = 0
+  , relations = M.empty
+  }
+
+mkRel :: MonadState HoareState m => Com -> Set Var -> m Prop
+mkRel c voc = do
+  HoareState count rels <- get
+  case M.lookup c rels of
+    Nothing -> do
+      let r = PRel ("$rel" ++ show count) (map V $ S.toList voc)
+      put (HoareState (count+1) (M.insert c r rels))
+      pure r
+    Just r -> pure r
+
+clause :: Prop -> Prop -> Prop
+clause pre post =
+  foldr PForall (PImpl pre post) (pvocab (PAnd pre post))
+
+hoare' :: (MonadState HoareState m, MonadWriter [Prop] m)
+      => Com
+      -> Prop {- The post condition -}
+      -> m Prop {- The pre condition -}
+hoare' c q =
+  case c of
+    Skip -> pure q
+    Prod{} -> do
+      let v = S.union (pvocab q) (cvocab c)
+      p <- mkRel c v
+      cart' p c Skip q
+      return p
+    c ->
+      cart c Skip q
+
+cart' :: (MonadState HoareState m, MonadWriter [Prop] m)
+      => Prop -> Com -> Com -> Prop -> m ()
+cart' p c0 c1 q =
+  case c0 of
+    Prod c0' c0'' -> do
+      cart' p c0' (mkProd c0'' c1) q
+      cart' p c0'' (mkProd c0' c1) q
+    c -> do
+      p' <- cart c c1 q
+      let v = S.union (pvocab p) (pvocab p')
+      tell [clause p p']
+
+cart :: (MonadState HoareState m, MonadWriter [Prop] m)
+     => Com -> Com -> Prop -> m Prop
+cart c0 c1 q =
+  case c0 of
+    Skip -> hoare' c1 q
+    Assign x e -> hoare' c1 (psubst x e q)
+    If e c0' c0'' -> do
+      q' <- hoare' (mkProd c0' c1) q
+      q'' <- hoare' (mkProd c0'' c1) q
+      let v = S.unions [pvocab q, cvocab c0, cvocab c1]
+      p <- mkRel (Prod c0 c1) v
+      tell [ clause (PAnd p e) q'
+           , clause (PAnd p (PNot e)) q''
+           ]
+      pure p
+    While{} -> undefined -- TODO
+    Seq c0' c0'' -> do
+      let v = S.unions [pvocab q, cvocab c0, cvocab c1]
+      p <- mkRel (Prod c0 c1) v
+      mapM_ (\(p0, p1) ->
+        when (p0 /= Skip && p1 /= Skip) $ do
+          p' <- hoare' p0 =<< hoare' p1 q
+          tell [clause p p']) (partitions (mkProd c0 c1))
+      pure p
+    Fail -> do
+      let v = pvocab q
+      p <- mkRel (Prod c0 c1) v
+      tell [clause PFalse q]
+      pure p
+    Prod{} -> undefined
+
+partitions :: Com -> [(Com, Com)]
+partitions = \case
+  Seq c0 c1 ->
+    S.toList $ S.fromList $ concat
+    [ [ (c0', mkSeq c0'' c1) | (c0', c0'') <- partitions c0 ]
+    , [ (mkSeq c0 c1', c1'') | (c1', c1'') <- partitions c1 ]
+    ]
+  Prod c0 c1 -> do
+    (p0, p0') <- partitions c0
+    (p1, p1') <- partitions c1
+    if or [ p0 == Skip && p1 == Skip
+          , p0' == Skip && p1' == Skip
+          , p0 == Skip && p1' == Skip
+          , p1 == Skip && p0' == Skip
+          ]
+    then []
+    else [(Prod p0 p1, Prod p0' p1')]
+  c -> [ (c, Skip), (Skip, c) ]
+
+mkSeq :: Com -> Com -> Com
+mkSeq Skip c = c
+mkSeq c Skip = c
+mkSeq c0 c1 = Seq c0 c1
+
+mkProd :: Com -> Com -> Com
+mkProd Skip c = c
+mkProd c Skip = c
+mkProd c0 c1 = Prod c0 c1
+
+hoare :: Com -> [Prop]
+hoare c = case runWriter (evalStateT (hoare' c PTrue) emptyHoareState) of
+            (p, ps) -> foldr PForall p (pvocab p) : ps
+
+test :: Com
+test =
+  Prod
+    ( Assign "a" (Lit 3)
+    `Seq` Assign "b" (Lit 5)
+    )
+    ( Assign "c" (Lit 5)
+    `Seq` Assign "d" (Lit 3)
+    )
+c0 :: Com
+c0 = Assign "a" (Lit 3) `Seq` Assign "b" (Lit 5)
+
+a, b :: Com
+a = Assign "a" (Lit 3)
+b = Assign "b" (Lit 5)
