proof/Proof1.v
@@ -32,32 +32,18 @@ Inductive com :=
 | cskip : com
 | cassign : nat -> aexpr -> com
 | cif : bexpr -> com -> com -> com
-| cwhile : nat -> bexpr -> com -> com
-(* | ccall : nat -> nat -> nat -> com *)
+| cwhile : bexpr -> com -> com
 | cseq : com -> com -> com
 | cprod : com -> com -> com.
 
 Notation "x '::=' a" := (cassign x a) (at level 60).
 
-Definition state' := nat -> nat.
+Definition state := nat -> nat.
 
-Inductive state :=
-| singleton : state' -> state
-| composite : state -> state -> state.
+Definition stempty : state := fun x => 0.
+Definition stupdate x n st : state := fun k => if k =? x then n else st k.
 
-Definition stempty : state' := fun x => 0.
-Definition stupdate x n st : state' := fun k => if k =? x then n else st k.
-
-Fixpoint stupdates xs ns st : state' :=
-  match xs with
-  | nil => st
-  | x :: xs => match ns with
-               | nil => st
-               | n :: ns => stupdates xs ns (stupdate x n st)
-               end
-  end.
-
-Fixpoint aeval (st:state') (e:aexpr) : nat :=
+Fixpoint aeval (st:state) (e:aexpr) : nat :=
   match e with
   | aop o e1 e2 => match o with
                    | oadd => aeval st e1 + aeval st e2
@@ -68,7 +54,7 @@ Fixpoint aeval (st:state') (e:aexpr) : nat :=
   | avar x => st x
   end.
 
-Fixpoint beval (st:state') (e:bexpr) : bool :=
+Fixpoint beval (st:state) (e:bexpr) : bool :=
   match e with
   | oop o e1 e2 => match o with
                    | oeq => aeval st e1 =? aeval st e2
@@ -89,53 +75,75 @@ Inductive ceval : com -> state -> state -> Prop :=
 | ESkip : forall st, ceval cskip st st
 | EAssign : forall st x e n,
     aeval st e = n ->
-    ceval (x ::= e) (singleton st) (singleton (stupdate x n st))
+    ceval (x ::= e) st (stupdate x n st)
 | EIfTrue : forall st st' e c1 c2,
     beval st e = true ->
-    ceval c1 (singleton st) (singleton st') ->
-    ceval (cif e c1 c2) (singleton st) (singleton st')
+    ceval c1 st st' ->
+    ceval (cif e c1 c2) st st'
 | EIfFalse : forall st st' e c1 c2,
     beval st e = false ->
-    ceval c2 (singleton st) (singleton st') ->
-    ceval (cif e c1 c2) (singleton st) (singleton st')
-| EWhileTrue : forall st st' st'' n e c,
+    ceval c2 st st' ->
+    ceval (cif e c1 c2) st st'
+| EWhileTrue : forall st st' st'' e c,
     beval st e = true ->
-    ceval c (singleton st) (singleton st') ->
-    ceval (cwhile n e c) (singleton st') (singleton st'') ->
-    ceval (cwhile (S n) e c) (singleton st) (singleton st'')
+    ceval c st st' ->
+    ceval (cwhile e c) st' st'' ->
+    ceval (cwhile e c) st st''
 | EWhileFalse : forall st e c,
     beval st e = false ->
-    ceval (cwhile 0 e c) (singleton st) (singleton st)
+    ceval (cwhile e c) st st
 | ESeq : forall st st' st'' c1 c2,
     ceval c1 st st' ->
     ceval c2 st' st'' ->
-    ceval (cseq c1 c2) st st''
-| EProd : forall st1 st1' st2 st2' c1 c2,
-    ceval c1 st1 st1' ->
-    ceval c2 st2 st2' ->
-    ceval (cprod c1 c2) (composite st1 st2) (composite st1' st2').
+    ceval (cseq c1 c2) st st''.
 Hint Constructors ceval.
+
+Inductive ieval : nat -> com -> state -> state -> Prop :=
+| ISkip : forall k st, ieval k cskip st st
+| IAssign : forall k st x e n,
+    aeval st e = n ->
+    ieval k (x ::= e) st (stupdate x n st)
+| IIfTrue : forall k st st' e c1 c2,
+    beval st e = true ->
+    ieval k c1 st st' ->
+    ieval k (cif e c1 c2) st st'
+| IIfFalse : forall k st st' e c1 c2,
+    beval st e = false ->
+    ieval k c2 st st' ->
+    ieval k (cif e c1 c2) st st'
+| IWhileTrue : forall k st st' st'' e c,
+    beval st e = true ->
+    ieval (S k) c st st' ->
+    ieval (S k) (cwhile e c) st' st'' ->
+    ieval k (cwhile e c) st st''
+| IWhileFalse : forall k st e c,
+    beval st e = false ->
+    ieval k (cwhile e c) st st
+| ISeq : forall k st st' st'' c1 c2,
+    ieval k c1 st st' ->
+    ieval k c2 st' st'' ->
+    ieval k (cseq c1 c2) st st''.
+Hint Constructors ieval.
 
 Definition Assertion := state -> Prop.
 Definition assert_implies (P Q : Assertion) : Prop :=
   forall st, P st -> Q st.
 
 Definition assn_sub x e P : Assertion :=
-  fun (st : state) => match st with
-  | singleton s => P (singleton (stupdate x (aeval s e) s))
-  | composite _ _ => False
-  end.
+  fun (st : state) => P (stupdate x (aeval st e) st).
 
 Definition triple (P:Assertion) (c:com) (Q:Assertion) : Prop :=
   forall st st', ceval c st st' -> P st -> Q st'.
 
 Notation "{{ P }} c {{ Q }}" := (triple P c Q) (at level 90, c at next level).
 
+Definition itriple (k:nat) (P:Assertion) (c:com) (Q:Assertion) : Prop :=
+  forall st st', ieval k c st st' -> P st -> Q st'.
+
+Notation "k |- {{ P }} c {{ Q }}" := (itriple k P c Q) (at level 90, c at next level).
+
 Definition bassn b : Assertion :=
-  fun st => match st with
-            | singleton s => (beval s b = true)
-            | composite _ _ => False
-            end.
+  fun st => beval st b = true.
 
 Theorem skip : forall P, {{P}} cskip {{P}}.
 Proof.
@@ -144,42 +152,109 @@ Proof.
   inversion H; subst; auto.
 Qed.
 
-Lemma while_unfold : forall n e c st st',
-  ceval (cwhile (S n) e c) (singleton st) (singleton st') <->
-  (ceval (cseq (cif e c cskip) (cwhile n e c)) (singleton st) (singleton st') /\ beval st e = true)
-.
+Lemma increase_depth : forall j k c st st',
+  j <= k ->
+  ieval j c st st' ->
+  ieval k c st st'.
 Proof.
-  split; intros.
-  - inversion H; subst.
-    split.
-    econstructor; try eassumption.
-    apply EIfTrue; eassumption.
-    assumption.
-  - inversion H; subst.
+  intros j k c.
+  induction c; intros; inversion H0; eauto.
+  - subst. admit.
+Admitted.
+
+Lemma iwhile_seq : forall P Q k c e,
+  S k |- {{P}} cseq (cif e c cskip) (cwhile e c) {{Q}} <->
+  k |- {{P}} cwhile e c {{Q}}.
+Proof.
+  split; unfold itriple; intros.
+  - eapply H.
     inversion H0; subst.
-    inversion H4; subst.
-    inversion H7; subst.
-    eapply EWhileTrue; eassumption.
-    eapply EWhileTrue; eassumption.
+    econstructor.
+    eapply IIfTrue; eauto.
+    eauto.
+    econstructor.
+    eapply IIfFalse; eauto.
+    inversion H0; subst.
+    apply increase_depth with k; eauto.
+    apply increase_depth with k; eauto.
+    eauto.
+  - inversion H0; subst.
+    eapply H.
+    inversion H5; subst.
+    eapply IWhileTrue; eauto.
+    inversion H11; subst.
+    inversion H8; subst.
     congruence.
+    eapply IWhileFalse. eauto.
+    eauto.
 Qed.
 
-
-Theorem while : forall P c0 n e,
-  ({{P}} cwhile n e c0 {{P}} ->
-   {{P}} cseq (cif e c0 cskip) (cwhile n e c0) {{P}}) ->
-  {{P}} cwhile (S n) e c0 {{P}}.
+Theorem iwhile : forall P k c e,
+  (S k |- {{P}} cwhile e c {{fun st => P st /\ not (bassn e st)}} ->
+   S k |- {{P}} cseq (cif e c cskip) (cwhile e c) {{fun st => P st /\ not (bassn e st)}}) ->
+  k |- {{P}} cwhile e c {{fun st => P st /\ not (bassn e st)}}.
 Proof.
-  induction n; unfold triple in *; intros.
-  - eapply H; intros.
-    + inversion H2; subst; assumption.
-    + econstructor.
-      eapply while_unfold in H0.
-      inversion H0; subst.
-      apply EIfTrue.
-      eapply H5.
+  unfold itriple in *; intros; induction k.
+  - admit.
+  - eapply IHk; intros.
+    eapply H; intros.
+    inversion H0; subst.
 
 
+Lemma while_unfold : forall n e c st st',
+  ceval (cwhile (S n) e c) st st' <->
+  beval st e = true /\ ceval (cseq c (cwhile n e c)) st st'.
+Proof.
+  split; intros.
+  - inversion H; subst; eauto.
+  - inversion H; subst; eauto.
+    inversion H1; subst.
+    econstructor; eauto.
+Qed.
+
+Lemma while_unfold_t : forall P Q n e c,
+  {{P}} cseq c (cwhile n e c) {{Q}} ->
+  {{P}} cwhile (S n) e c {{Q}}.
+Proof.
+  unfold triple; intros.
+  eapply H.
+  rewrite while_unfold in H0.
+  inversion H0; subst; clear H0.
+  inversion H3; subst; clear H3.
+  econstructor; eauto.
+  eauto.
+Qed.
+
+Theorem hoare_seq : forall P Q R c0 c1,
+  {{P}} c0 {{R}} ->
+  {{R}} c1 {{Q}} ->
+  {{P}} cseq c0 c1 {{Q}}.
+Admitted.
+
+
+Theorem while : forall P n c e,
+  ({{P}} cwhile n e c {{fun st => P st /\ not (bassn e st)}} ->
+   {{P}} cseq c (cwhile n e c) {{fun st => P st /\ not (bassn e st)}}) ->
+  {{P}} cwhile (S n) e c {{fun st => P st /\ not (bassn e st)}}.
+Proof.
+  intros.
+  induction n.
+  - unfold triple in *; intros; rewrite while_unfold in H0.
+    inversion H0.
+    eapply H; intros; eauto.
+    + inversion H4; subst.
+      split; auto; try congruence.
+  - apply while_unfold_t.
+    eapply hoare_seq.
+    + admit.
+    + apply IHn.
+    ther-
+    + unfold triple in *; intros.
+      eapply H; intros.
+      eapply IHn; intros.
+    a
+
+Qed.
 
 Theorem consequence : forall P P' Q Q' c,
   assert_implies P P' ->
