proof/Example.v
@@ -1,0 +1,879 @@
+Require Import Omega.
+
+(* preliminary definitions and lemmas *)
+
+Require Import String.
+Require Import OrderedType.
+
+Declare Module String_as_OT : OrderedType
+    with Definition t := string
+    with Definition eq := @eq string.
+
+Require Import Ensembles.
+
+Arguments Union [_] _ _ _.
+Arguments Empty_set [_] _.
+Arguments Singleton [_] _ _.
+Arguments In [_] _ _.
+
+Section BIGCUP.
+
+Context {A : Type}.
+
+Fixpoint BIGCUP (n : nat) (f : nat -> A) : Ensemble A :=
+  match n with
+  | O => Singleton (f 0)
+  | S m => Union (Singleton (f n)) (BIGCUP m f)
+  end.
+
+Variable f : nat -> A.
+
+Lemma In_BIGCUP X n : n <= X -> In (BIGCUP X f) (f n).
+Proof.
+  induction X.
+    destruct n; [intros _| now auto].
+    simpl.
+    now apply In_singleton.
+  intros.
+  simpl.
+  rewrite PeanoNat.Nat.le_succ_r in H.
+  destruct H as [nX | ?]; [ | subst n].
+    now apply Union_intror, IHX.
+    now apply Union_introl, In_singleton.
+Qed.
+
+Lemma In_BIGCUP_inv t X : In (BIGCUP X f) t -> exists n, n <= X /\ t = f n.
+Proof.
+  induction X.
+    simpl.
+    inversion_clear 1.
+    now exists 0.
+  simpl.
+  inversion_clear 1.
+    exists (S X).
+    split; [ now auto | ].
+    now inversion_clear H0.
+  destruct (IHX H0) as [n [nX tfn]].
+  exists n.
+  split; [ | now auto].
+  now apply le_S.
+Qed.
+
+End BIGCUP.
+
+Require Import FMapList.
+Require FMapFacts.
+
+Module Type STATE.
+
+Parameter state : Set.
+Definition assert := state -> Prop.
+Definition entails (P Q : assert) : Prop := forall s, P s -> Q s.
+Parameter exp : Set.
+Parameter bexp : Set.
+Parameter eval : exp -> state -> nat.
+Parameter beval : bexp -> state -> Prop.
+
+End STATE.
+
+Module Type CMD0 (S : STATE).
+
+Parameter cmd0 : Set.
+Parameter exec0 : S.state -> cmd0 -> S.state -> Prop.
+Parameter hoare0 : S.assert -> cmd0 -> S.assert -> Prop.
+
+End CMD0.
+
+Module Procs := FMapList.Make (String_as_OT).
+Module ProcsFacts := FMapFacts.Facts Procs.
+
+Definition proc := Procs.key.
+
+Module Cmd (S : STATE) (Cmd0 : CMD0 S).
+
+Let state := S.state.
+Let exp := S.exp.
+Let bexp := S.bexp.
+
+Let assert := S.state -> Prop.
+
+Local Notation "P ===> Q" := (S.entails P Q) (at level 89, no associativity).
+
+Let beval := S.beval.
+
+Local Notation "'[' e ']b_' s" := (beval e s) (at level 9, format "'[' [  e  ]b_ s ']'", no associativity).
+
+Inductive cmd : Type :=
+| basic : Cmd0.cmd0 -> cmd
+| seq : cmd -> cmd -> cmd
+| ifte : bexp -> cmd -> cmd -> cmd
+| call : proc -> cmd.
+
+Local Notation "c .; d" := (seq c d) (at level 81, right associativity).
+
+Local Notation "'If' e 'Then' c1 'Else' c2" := (ifte e c1 c2)
+  (at level 200, right associativity, format
+"'[v' '[' 'If'  e  'Then' ']' '//'   '[' c1 ']' '//' '[' 'Else' ']' '//'   '[' c2 ']' '//' ']'").
+
+Definition procs := Procs.t cmd.
+
+Reserved Notation "l |~ s >- c ---> t" (at level 70, s, c, t at next level, no associativity).
+
+Inductive exec (l : procs) : state -> cmd -> state -> Prop :=
+| exec_basic : forall s c0 s1, Cmd0.exec0 s c0 s1 ->
+  l |~ s >- basic c0 ---> s1
+| exec_seq : forall s s1 s2 c d,
+  l |~ s >- c ---> s1 -> l |~ s1 >- d ---> s2 ->
+  l |~ s >- c .; d ---> s2
+| exec_ifte_true : forall s s1 b c d, [ b ]b_ s ->
+  l |~ s >- c ---> s1 -> l |~ s >- If b Then c Else d ---> s1
+| exec_ifte_false : forall s s1 b c d, ~ [ b ]b_ s ->
+  l |~ s >- d ---> s1 -> l |~ s >- If b Then c Else d ---> s1
+| exec_call : forall s s1 p c, Procs.MapsTo p c l ->
+  l |~ s >- c ---> s1 -> l |~ s >- call p ---> s1
+(* | exec_call_err : forall s p, *)
+(*   Procs.find p l = None -> *)
+(*   l |~ s >- call p ---> None *)
+where "l |~ s >- c ---> t" := (exec l s c t).
+
+Reserved Notation "l '|~' s '>-' c '-^' n '->' t" (at level 70, s, c, n, t at next level, no associativity).
+
+(* Indexed execution -- some call depth `n` *)
+Inductive iexec (l : procs) : nat -> state -> cmd -> state -> Prop :=
+| iexec_cmd0 : forall n s c s1, Cmd0.exec0 s c s1 -> l |~ s >- basic c -^ n -> s1
+| iexec_seq : forall n s s1 s2 c d,
+  l |~ s >- c -^ n -> s1 -> l |~ s1 >- d -^ n -> s2 -> l |~ s >- c .; d -^ n -> s2
+| iexec_ifte_true : forall n s s1 b c d, [ b ]b_ s ->
+  l |~ s >- c -^ n -> s1 ->
+  l |~ s >- If b Then c Else d -^ n -> s1
+| iexec_ifte_false : forall n s s1 b c d, ~ [ b ]b_ s ->
+  l |~ s >- d -^ n -> s1 ->
+  l |~ s >- If b Then c Else d -^ n -> s1
+| iexec_call : forall n s s1 p c,
+    Procs.MapsTo p c l ->
+    l |~ s >- c -^ n -> s1 ->
+    l |~ s >- call p -^ S n -> s1
+(* | iexec_call_err : forall n s p, *)
+(*     Procs.find p l = None -> *)
+(*     l |~ s >- call p -^ S n -> None *)
+where "l '|~' s >- c '-^' n '->' t" := (iexec l n s c t).
+
+Lemma iexec_S n l s prg s1 :
+  l |~ s >- prg -^ n -> s1 ->
+  forall m, n <= m -> l |~ s >- prg -^ m -> s1.
+Proof.
+  induction 1; intros m nm.
+  - now constructor.
+  - apply iexec_seq with s1; now auto.
+  - apply iexec_ifte_true; now auto.
+  - apply iexec_ifte_false; now auto.
+  - destruct m as [| m]; [now inversion nm | ].
+    apply iexec_call with c; [now auto |].
+    apply IHiexec.
+    now apply Le.le_S_n.
+Qed.
+
+Lemma iexec_exec n l s c t : l |~ s >- c -^ n -> t -> l |~ s >- c ---> t.
+Proof.
+  induction 1.
+  - now apply exec_basic.
+  - now apply exec_seq with s1.
+  - now apply exec_ifte_true.
+  - now apply exec_ifte_false.
+  - now apply exec_call with c.
+Qed.
+
+Lemma iexec_incr l n s s1 c :
+  l |~ s >- c -^ n -> s1 ->
+  forall m, n <= m ->
+  l |~ s >- c -^ m -> s1.
+Proof.
+  induction 1; intros m nm.
+  - now apply iexec_cmd0.
+  - apply iexec_seq with s1.
+    now apply IHiexec1.
+    now apply IHiexec2.
+  - apply iexec_ifte_true; [now auto |].
+    now apply IHiexec.
+  - apply iexec_ifte_false; [now auto|].
+    now apply IHiexec.
+  - destruct m; [omega | ].
+    apply iexec_call with c; [now auto | ].
+    apply IHiexec; omega.
+Qed.
+
+Lemma iexec_seq_exists l n1 s s1 c :
+  l |~ s >- c -^ n1 -> s1 ->
+  forall n2 d s2,
+  l |~ s1 >- d -^ n2 -> s2 ->
+  exists n, l |~ s >- c .; d -^ n -> s2.
+Proof.
+  intros Hc n2 d s2 Hd.
+  exists (max n1 n2).
+  apply iexec_seq with s1.
+    apply iexec_incr with n1; [now auto |].
+    now apply Max.le_max_l.
+  apply iexec_incr with n2; [now auto |].
+  now apply Max.le_max_r.
+Qed.
+
+Lemma exec_iexec l s c t : l |~ s >- c ---> t -> exists n, l |~ s >- c -^ n -> t.
+Proof.
+  induction 1.
+  - exists O.
+    now apply iexec_cmd0.
+  - destruct IHexec1 as [n1 IH1].
+    destruct IHexec2 as [n2 IH2].
+    now eapply iexec_seq_exists; eauto.
+  - destruct IHexec as [n IH].
+    exists n.
+    now apply iexec_ifte_true.
+  - destruct IHexec as [n IH].
+    exists n.
+    now apply iexec_ifte_false.
+  - destruct IHexec as [n IH].
+    exists (S n).
+    now apply iexec_call with c.
+Qed.
+
+Record spec := Spec {
+  pre : assert ;
+  callee : proc ;
+  post : assert}.
+
+Reserved Notation "l \^ E |~{[ P ]} c {[ Q ]}"
+  (at level 70, E, P, c, Q at next level, no associativity, format "l  \^  E  |~{[  P  ]}  c  {[  Q  ]}").
+
+Inductive hoare (l  : procs) : Ensemble spec -> assert -> cmd -> assert -> Prop :=
+| hoare_basic : forall E P Q c, Cmd0.hoare0 P c Q ->
+  l \^ E |~{[ P ]} basic c {[ Q ]}
+| hoare_seq : forall E P Q R c d,
+  l \^ E |~{[ P ]} c {[ Q ]} -> l \^ E |~{[ Q ]} d {[ R ]} ->
+  l \^ E |~{[ P ]} c .; d {[ R ]}
+| hoare_conseq : forall E c (P Q : assert),
+  (forall s, P s -> exists P' Q',
+    l \^ E |~{[ P' ]} c {[ Q' ]} /\ P' s /\ (Q' ===> Q)) ->
+  l \^ E |~{[ P ]} c {[ Q ]}
+| hoare_ifte : forall E P Q b c d,
+  l \^ E |~{[ fun s => P s /\ [ b ]b_ s ]} c {[ Q ]} ->
+  l \^ E |~{[ fun s => P s /\ ~ [ b ]b_ s ]} d {[ Q ]} ->
+  l \^ E |~{[ P ]} If b Then c Else d {[ Q ]}
+| hoare_call : forall E P Q p E',
+  In E' (Spec P p Q) ->
+  (forall t, In E' t -> exists c, Procs.MapsTo (callee t) c l /\
+     l \^ Union E E' |~{[ pre t ]} c {[ post t ]}) ->
+  l \^ E |~{[ P ]} call p {[ Q ]}
+| hoare_call2 : forall E P Q p, In E (Spec P p Q) ->
+  l \^ E |~{[ P ]} call p {[ Q ]}
+where "l \^ E |~{[ P ]} c {[ Q ]}" := (hoare l E P c Q).
+
+(* usual consequence lemmas *)
+
+Lemma hoare_conseq_spec l E P P' Q Q' c : P ===> P' -> Q' ===> Q ->
+  l \^ E |~{[ P' ]} c {[ Q' ]} -> l \^ E |~{[ P ]} c {[ Q ]}.
+Proof.
+  intros.
+  apply hoare_conseq.
+  intros s Ps.
+  exists P', Q'; split; [assumption | ].
+  split; [ | assumption].
+  now apply H.
+Qed.
+
+Lemma hoare_stren l E P P' Q c : P ===> P' ->
+  l \^ E |~{[ P' ]} c {[ Q ]} -> l \^ E |~{[ P ]} c {[ Q ]}.
+Proof.
+  intros.
+  apply hoare_conseq_spec with P' Q; auto.
+  now intuition.
+Qed.
+
+Lemma hoare_weak l E P Q Q' c : Q' ===> Q ->
+  l \^ E |~{[ P ]} c {[ Q' ]} -> l \^ E |~{[ P ]} c {[ Q ]}.
+Proof.
+  intros.
+  apply hoare_conseq_spec with P Q'; auto.
+  now intuition.
+Qed.
+
+Lemma hoare_ind2 : forall l (G : Ensemble spec -> assert -> cmd -> assert -> Prop),
+ (forall E P Q c, Cmd0.hoare0 P c Q -> G E P (basic c) Q) ->
+ (forall E P Q R c d, l \^ E |~{[ P ]} c {[ Q ]} ->
+   G E P c Q -> l \^ E |~{[ Q ]} d {[ R ]} -> G E Q d R -> G E P (c.; d) R) ->
+ (forall E c (P Q : assert) ,
+   (forall s, P s ->
+   exists P' Q', G E P' c Q' /\ (*l \^ E |~{[ P']} c {[Q']} /\*) P' s /\ (Q' ===> Q)) ->
+     G E P c Q) ->
+ (forall E (P : state -> _) Q b c d,
+  l \^ E |~{[ fun s => P s /\ [ b ]b_ s ]} c {[Q]} ->
+  G E (fun s => P s /\ [ b ]b_ s) c Q ->
+  l \^ E |~{[ fun s => P s /\ ~ [ b ]b_ s ]} d {[Q]} ->
+  G E (fun s => P s /\ ~ [ b ]b_ s) d Q ->
+  G E P (If b Then c Else d) Q) ->
+  (forall E P Q p E',
+    In E' (Spec P p Q) ->
+    (forall t0,
+     In E' t0 -> exists c,
+       Procs.MapsTo (callee t0) c l /\ (* l \^ Union E E' |~{[ C.fpre t0]} pro {[C.fpost t0]}*)
+       G (Union E E') (pre t0) c (post t0)) ->
+   G E P (call p) Q) ->
+  (forall E P Q p,
+   In E (Spec P p Q) -> G E P (call p) Q) ->
+  forall E P c Q, l \^ E |~{[ P ]} c {[ Q ]} -> G E P c Q.
+Proof.
+  (* induction w.r.t. l \^ E |~{[ P ]} c {[ Q ]} *)
+  fix 13.
+  intros.
+  destruct H5.
+  - now apply H.
+  - apply H0 with Q; try auto.
+    apply hoare_ind2 with l; try auto.
+    apply hoare_ind2 with l; try auto.
+  - apply H1; try auto.
+    intros s P0s.
+    destruct (H5 _ P0s) as [P' [Q' K]].
+    exists P', Q'.
+    split.
+    apply hoare_ind2 with l; try auto.
+    tauto.
+    tauto.
+  - apply H2; try auto.
+    apply hoare_ind2 with l; try auto.
+    apply hoare_ind2 with l; try auto.
+  - apply H3 with E'; try auto.
+    intros t0 Ht0.
+    destruct (H6 _ Ht0) as [pro [Hpro1 Hpro2]].
+    exists pro.
+    split; [now auto | ].
+    now apply hoare_ind2 with l; try auto.
+  - now apply H4.
+Qed.
+
+Definition hoare_sem l P c (Q : assert) : Prop :=
+  forall s s1, P s -> l |~ s >- c ---> s1 -> Q s1.
+
+Local Notation "l |={{ P }} c {{ Q }}" := (hoare_sem l P c Q)
+  (at level 70, P, c, Q at next level, format "l  |={{  P  }}  c  {{  Q  }}").
+
+Definition hoare_sem_ctxt l E P c Q :=
+  (forall t, In E t -> l |={{ pre t }} call (callee t) {{ post t }}) ->
+  l |={{ P }} c {{ Q }}.
+
+Local Notation "l \^ E |={{ P }} c {{ Q }}" := (hoare_sem_ctxt l E P c Q)
+  (at level 70, E, P, c, Q at next level, format "l  \^  E  |={{  P  }}  c  {{  Q  }}").
+
+Definition hoare_sem_n l n P c (Q : assert) : Prop :=
+    forall s s1, P s -> l |~ s >- c -^ n -> s1 -> Q s1.
+
+Local Notation "l |= n {{ P }} c {{ Q }}" := (hoare_sem_n l n P c Q)
+  (at level 70, n, P, c, Q at next level, format "l  |=  n  {{  P  }}  c  {{  Q  }}").
+
+Lemma hoare_sem_Sn n P l prg Q : l |= S n {{ P }} prg {{ Q }} ->
+  l |= n {{ P }} prg {{ Q }}.
+Proof.
+  unfold hoare_sem_n.
+  intros H s Ps.
+  intros ? ?.
+  apply H with s.
+  apply X.
+  apply iexec_S with n; [now auto| omega].
+Qed.
+
+Lemma hoare_sem_n_sem l P c Q :
+  l |={{ P }} c {{ Q }} <-> forall n, l |= n {{ P }} c {{ Q }}.
+Proof.
+  unfold hoare_sem_n, hoare_sem; split; intros H.
+  - intros n s s1 Ps Psh1.
+    apply H with s; auto.
+    now apply iexec_exec with n.
+  - intros s s1 Ps abs.
+    destruct (exec_iexec _ _ _ _ abs) as [n IH].
+    eapply H; eauto.
+Qed.
+
+Definition hoare_sem_ctxt_n l E n P c Q :=
+  (forall t, In E t -> l |= n {{ pre t }} call (callee t) {{ post t }}) ->
+  l |= n {{ P }} c {{ Q }}.
+
+Local Notation "l \^ E |= n {{ P }} c {{ Q }}" := (hoare_sem_ctxt_n l E n P c Q)
+  (at level 70, E, n, P, c, Q at next level, format "l  \^  E  |=  n  {{  P  }}  c  {{  Q  }}").
+
+Lemma hoare_sem_ctxt_n_sem_ctxt l E P c Q :
+  (forall n, l \^ E |= n {{ P }} c {{ Q }}) ->
+  l \^ E |={{ P }} c {{ Q }}.
+Proof.
+  unfold hoare_sem_ctxt_n, hoare_sem_ctxt; intros H K.
+  apply hoare_sem_n_sem; intros n.
+  apply H; intros t Ht.
+  apply hoare_sem_n_sem.
+  now apply K.
+Qed.
+
+Lemma hoare_sound_n E P Q l c :
+  (forall P Q l c, Cmd0.hoare0 P c Q -> forall n, l |= n {{ P }} basic c {{ Q }}) ->
+  l \^ E |~{[ P ]} c {[ Q ]} -> forall n, l \^ E |= n {{ P }} c {{ Q }}.
+Proof.
+  intro Hcmd0.
+  induction 1 using hoare_ind2.
+  - intros n Hn.
+    now apply Hcmd0.
+  - intros n Hn s s1 Ps.
+    inversion_clear 1.
+    eapply IHhoare2; intros. intro. intros.
+    eapply Hn; eauto.
+    eapply IHhoare1; intros. intro. intros.
+    eapply Hn; eauto.
+    apply Ps.
+    eauto.
+    eauto.
+  - intros n Hn s s1 Ps.
+    destruct (H _ Ps) as [P' [Q' [IH1 [IH2 IH3]]]].
+    intro. intros.
+    apply IH3.
+    eapply IH1. intros; intro; intros.
+    eapply Hn; eauto.
+    eauto.
+    eauto.
+  - intros n Hn s s1 Ps.
+    inversion_clear 1.
+    eapply IHhoare1. intros; intro; intros.
+    eapply Hn; eauto.
+    eauto.
+    eauto.
+    eapply IHhoare2. intros; intro; intros.
+    eapply Hn; eauto.
+    eauto.
+    eauto.
+  - (* case call *) intro n.
+    unfold hoare_sem_ctxt_n.
+    (* generalization *)
+    cut ((forall t,
+      In E t -> l |= n {{ pre t }} call (callee t) {{ post t }}) ->
+      forall P' Q' p,
+      In E' (Spec P' p Q') -> l |= n {{ P' }} call p {{ Q' }}).
+      intros G H_.
+      now apply G.
+    induction n.
+    + (* n = 0 *) intros nis0 P' Q' p' p'_E'.
+      unfold hoare_sem_n.
+      intros s s1 P's. inversion 1.
+    + (* n > 0 *) intros nisSn P' Q' p' p'_E'.
+      assert (nisn : forall t, In E t ->
+        l |= n {{ pre t }} call (callee t) {{ post t }}).
+        intros t' t'_E.
+        apply hoare_sem_Sn.
+        now apply nisSn.
+      clear nisSn.
+      assert (IHn_ : forall t, In E' t ->
+         exists c, Procs.MapsTo (callee t) c l /\
+          l |= n {{ pre t }} c {{ post t }}).
+        intros t' t'_E'.
+        destruct (H0 _ t'_E') as [c [H01 H02]].
+        exists c.
+        split; [now auto|].
+        apply H02.
+        intros t''.
+        inversion_clear 1.
+          now apply nisn.
+        apply (IHn nisn).
+        now destruct t''.
+      clear nisn IHn.
+      destruct (IHn_ _ p'_E') as [c [c_l Hc]].
+      clear IHn_.
+      intros s s1 P1.
+      red in Hc.
+      intro.
+      apply Hc with s s1 in P1.
+      apply P1.
+      eapply H0.
+      apply Hc with s s1 in P1.
+      eapply c_l.
+      simpl.
+      intros.
+      destruct P1 as [P1' P1''].
+      split.
+      * contradict P1'.
+        inversion_clear P1'.
+          generalize (ProcsFacts.MapsTo_fun H1 c_l); intro c0_c.
+          now rewrite <- c0_c.
+        (* apply Procs.find_1 in c_l. *)
+        (* simpl in c_l. *)
+        (* now rewrite c_l in H1. *)
+      * intros s.
+        inversion_clear 1.
+        generalize (ProcsFacts.MapsTo_fun H2 c_l); intros ?; subst c.
+        now apply P1'' in H3.
+  - intros n Hn.
+    generalize (Hn _ H).
+    intros Ht s Ps.
+    split.
+    + generalize (Ht _ Ps).
+      now inversion_clear 1.
+    + intros s1.
+      exact (proj2 (Ht _ Ps) s1).
+Qed.
+
+Lemma hoare_sound E P Q l c :
+  (forall P Q l c, Cmd0.hoare0 P c Q -> l |={{ P }} basic c {{ Q }}) ->
+  l \^ E |~{[ P ]} c {[ Q ]} -> l \^ E |={{ P }} c {{ Q }}.
+Proof.
+  intros.
+  apply hoare_sem_ctxt_n_sem_ctxt; intros n.
+  apply hoare_sound_n; [| assumption].
+  intros.
+  now apply hoare_sem_n_sem, H.
+Qed.
+
+End Cmd.
+
+(* expression language *)
+
+Module Vars := FMapList.Make (String_as_OT).
+
+Module VarsFacts := FMapFacts.Facts Vars.
+
+Definition var := Vars.key.
+
+Inductive exp :=
+| exp_var : var -> exp
+| add : exp -> exp -> exp
+| mul : exp -> exp -> exp
+| sub : exp -> exp -> exp
+| cst : nat -> exp.
+
+Coercion cst : nat >-> exp.
+
+Notation "% v" := (exp_var v) (at level 4).
+Notation "a \- b" := (sub a b) (at level 65).
+Notation "a \+ b" := (add a b) (at level 65).
+Notation "a \* b" := (mul a b) (at level 58).
+
+Inductive bexp :=
+| equa : exp -> exp -> bexp
+| neg : bexp -> bexp.
+
+Notation "a \= b" := (equa a b) (at level 64).
+Notation "a \!= b" := (neg (equa a b)) (at level 64).
+
+Module state <: STATE.
+
+Definition state := Vars.t nat.
+Definition assert := state -> Prop.
+Definition entails (P Q : assert) : Prop := forall s, P s -> Q s.
+Definition exp := exp.
+Definition bexp := bexp.
+Fixpoint eval e s :=
+  match e with
+  | % v => match Vars.find v s with Some x => x | _ => 0 end
+  | e1 \+ e2 => eval e1 s + eval e2 s
+  | e1 \* e2 => eval e1 s * eval e2 s
+  | e1 \- e2 => eval e1 s - eval e2 s
+  | cst c => c
+  end.
+
+Fixpoint beval b s :=
+  match b with
+    | e1 \= e2 => eval e1 s = eval e2 s
+    | neg b => ~ beval b s
+  end.
+
+Definition upd v (n : nat) s := Vars.add v n s.
+
+Local Notation "'[' e ']_' s" := (state.eval e s) (at level 9, format "'[' [  e  ]_ s ']'", no associativity).
+
+Lemma eval_upd_same str v s : [ % str ]_(state.upd str v s) = v.
+Proof.
+unfold state.eval at 1.
+rewrite VarsFacts.add_eq_o; now auto.
+Qed.
+
+Lemma eval_upd_diff str str' v s : str <> str' -> [ % str ]_(state.upd str' v s) = [ % str ]_s.
+Proof.
+intros H.
+unfold state.eval at 1.
+rewrite VarsFacts.add_neq_o; now auto.
+Qed.
+
+End state.
+
+Notation "P ===> Q" := (state.entails P Q) (at level 89, no associativity) : hoare_scope.
+
+Arguments state.eval e s : simpl never.
+
+Notation "'[' e ']_' s" := (state.eval e s) (at level 9, format "'[' [  e  ]_ s ']'", no associativity).
+
+Notation "'[' e ']b_' s" := (state.beval e s) (at level 9, format "'[' [  e  ]b_ s ']'", no associativity) : hoare_scope.
+
+Module cmd0 <: CMD0 state.
+
+Inductive cmd0' :=
+| assign : var -> state.exp -> cmd0'.
+Definition cmd0 := cmd0'.
+
+Local Notation "x <- e" := (cmd0.assign x e) (at level 80).
+
+Inductive exec0' : state.state -> cmd0 -> option state.state -> Prop :=
+| exec0_assign : forall s v e, exec0' s (v <- e) (Some (state.upd v ([ e ]_s) s)).
+Definition exec0 := exec0'.
+
+Inductive wp_assign v e P : state.assert :=
+| wp_assign_c : forall s, P (state.upd v ([ e ]_s) s) -> wp_assign v e P s.
+
+Inductive hoare0' : state.assert -> cmd0 -> state.assert -> Prop :=
+| hoare0_assign : forall Q v e, hoare0' (wp_assign v e Q) (v <- e) Q.
+Definition hoare0 := hoare0'.
+
+End cmd0.
+
+Notation "x <- e" := (cmd0.assign x e) (at level 80) : hoare_scope.
+
+Module C := Cmd state cmd0.
+
+Coercion cmd0_cmd (c : cmd0.cmd0') : C.cmd := C.basic c.
+
+Notation "c .; d" := (C.seq c d) (at level 81, right associativity, format "'[v' c '.;' '//' d ']'") : hoare_scope.
+
+Notation "'If' e 'Then' c1 'Else' c2" := (C.ifte e c1 c2)
+  (at level 200, right associativity, format
+"'[v' '[' 'If'  e  'Then' ']' '//'   '[' c1 ']' '//' '[' 'Else' ']' '//'   '[' c2 ']' '//' ']'") : hoare_scope.
+
+Notation "l '|~' s '>-' c '-^' n '->' t" := (C.iexec l n s c t)
+  (at level 70, s, c, n, t at next level, no associativity) : hoare_scope.
+
+Notation "l |={{ P }} c {{ Q }}" := (C.hoare_sem l P c Q)
+  (at level 70, P, c, Q at next level, format "l  |={{  P  }}  c  {{  Q  }}") : hoare_scope.
+
+Local Open Scope hoare_scope.
+
+Lemma sound0 P Q l c : cmd0.hoare0 P c Q -> l |={{ P }} C.basic c {{ Q }}.
+Proof.
+induction 1.
+unfold C.hoare_sem.
+intros s H.
+split.
+- inversion_clear 1.
+  now inversion H1.
+- intros ?.
+  inversion_clear 1.
+  inversion_clear H1.
+  now inversion_clear H.
+Qed.
+
+Notation "l \^ E |= n {{ P }} c {{ Q }}" := (C.hoare_sem_ctxt_n l E n P c Q)
+  (at level 70, E, n, P, c, Q at next level, format "l  \^  E  |=  n  {{  P  }}  c  {{  Q  }}") : hoare_scope.
+
+Notation "l \^ E |~{[ P ]} c {[ Q ]}" := (C.hoare l E P c Q)
+  (at level 70, E, P, c, Q at next level, no associativity,
+  format "l  \^  E  |~{[  P  ]}  c  {[  Q  ]}") : hoare_scope.
+
+Notation "l |={{ P }} c {{ Q }}" := (C.hoare_sem l P c Q) (at level 70, P, c, Q at next level,
+  format "l  |={{  P  }}  c  {{  Q  }}") : hoare_scope.
+
+Notation "l \^ E |={{ P }} c {{ Q }}" := (C.hoare_sem_ctxt l E P c Q)
+  (at level 70, E, P, c, Q at next level, format "l \^ E |={{  P  }}  c  {{  Q  }}").
+
+Notation "l |~ s >- c ---> t" := (C.exec l s c t) (at level 70, s, c, t at next level, no associativity).
+
+(** Example *)
+
+Require Import Factorial.
+
+Lemma fact_fact n : 1 <= n -> fact (n - 1) * n = fact n.
+Proof.
+destruct n; [omega | intros _].
+simpl.
+rewrite Nat.sub_0_r, Nat.mul_succ_r, Nat.mul_comm.
+omega.
+Qed.
+
+Module FactorialWhile.
+
+Definition facto :=
+  (C.while (% "x" \!= 0)
+    ("ret" <- % "ret" \* % "x" .;
+     "x" <- % "x" \- 1))%string.
+
+Lemma facto_fact X :
+  (Procs.empty _ \^
+  @Empty_set _
+  |~{[ fun s => [% "x" ]_s = X /\ [% "ret" ]_s = 1 ]}
+  facto
+  {[ fun s => [ % "ret" ]_ s = fact X ]})%string.
+Proof.
+apply C.hoare_stren with (fun s =>
+  [ % "ret" ]_ s * fact ([ % "x" ]_ s) = fact X)%string.
+  intros s [H1 H2].
+  rewrite H1, H2.
+  omega.
+apply C.hoare_weak with (fun s =>
+  ([ % "ret" ]_ s * fact ([ % "x" ]_ s) = fact X ) /\
+  ~ [ % "x" \!= 0 ]b_ s)%string.
+  intros s [H1 H2].
+  assert (H3 : [ % "x"%string ]_s = 0).
+    unfold state.eval in H2.
+    simpl in H2.
+    unfold state.eval at 2 in H2.
+    omega.
+  rewrite <- H1.
+  rewrite H3.
+  simpl.
+  omega.
+apply C.hoare_while.
+apply C.hoare_seq with (fun s =>
+  [ % "ret" ]_ s * fact ([ % "x" ]_ s - 1) = fact X /\ 0 <= [ % "x" ]_ s - 1)%string.
+  apply C.hoare_stren with (cmd0.wp_assign "ret"%string (% "ret"%string \* % "x"%string) (fun s =>
+                                                [ % "ret"%string ]_s *
+                                                fact ([ % "x"%string ]_s - 1) =
+                                                fact X /\
+                                                0 <= [ % "x"%string ]_s - 1)).
+    intros s [H1 H2].
+    apply cmd0.wp_assign_c.
+    rewrite state.eval_upd_same.
+    rewrite state.eval_upd_diff; [|now auto].
+    unfold state.eval at 1.
+    simpl in H2.
+    unfold state.eval at 2 in H2.
+    fold ([ % "x"%string ]_ s).
+    fold ([ % "ret"%string ]_ s).
+    split; [ | omega].
+    rewrite <- mult_assoc.
+    rewrite (mult_comm [% "x"%string]_s).
+    rewrite fact_fact; [ | omega].
+    now rewrite H1.
+  apply C.hoare_basic.
+  now apply cmd0.hoare0_assign.
+apply C.hoare_stren with (cmd0.wp_assign "x"%string  (% "x"%string \- 1) (fun s =>
+   [ % "ret"%string ]_s * fact [ % "x"%string ]_s = fact X)).
+  intros s [H1 H2].
+  apply cmd0.wp_assign_c.
+  rewrite state.eval_upd_diff; [| now auto].
+  rewrite state.eval_upd_same.
+  now auto.
+apply C.hoare_basic.
+now apply cmd0.hoare0_assign.
+Qed.
+
+End FactorialWhile.
+
+Module FactorialRec.
+
+Definition facto : C.cmd :=
+  (If (% "x" \= 0) Then
+    "ret" <- 1
+  Else
+   "x" <- % "x" \- 1 .;
+   C.call "facto" .;
+   "x" <- % "x" \+ 1 .;
+   "ret" <- % "ret" \* % "x")%string.
+
+Definition factospec x := (C.Spec
+  (fun s => [ %"x" ]_s = x)
+  "facto"
+  (fun s => [ %"x" ]_s = x /\ [ % "ret" ]_ s = fact x))%string.
+
+Lemma facto_fact X :
+  (Procs.add "facto" facto (Procs.empty _) \^
+  @Empty_set _
+  |~{[ fun s => [% "x" ]_s = X ]}
+  C.call "facto"
+  {[ fun s => [% "x" ]_s = X /\ [ % "ret" ]_ s = fact X ]})%string.
+Proof.
+(* call facto *)
+apply C.hoare_call with (E' := BIGCUP X factospec).
+  now apply (In_BIGCUP factospec).
+intros t InSpecs.
+destruct (In_BIGCUP_inv _ _ _ InSpecs) as [n [nX tn]].
+exists facto.
+rewrite tn.
+clear InSpecs tn.
+split.
+  now apply Procs.add_1.
+unfold facto at 2.
+(* if x = 0 then ... else ... *)
+apply C.hoare_ifte.
+  apply C.hoare_stren with (cmd0.wp_assign "ret"%string 1 (C.post (factospec n))).
+    intros s.
+    simpl.
+    destruct 1 as [xn x0].
+    unfold state.eval at 2 in x0.
+    subst n.
+    apply cmd0.wp_assign_c.
+    rewrite state.eval_upd_diff; [ | now auto].
+    rewrite state.eval_upd_same.
+    now rewrite x0.
+  apply C.hoare_basic.
+  now apply cmd0.hoare0_assign.
+simpl.
+(* x <- x - 1; call; ... *)
+apply C.hoare_seq with (fun s => [% "x"%string ]_s = n - 1 /\ 1 <= n).
+  apply C.hoare_stren with (cmd0.wp_assign "x" (% "x" \- 1) (fun s => [ % "x" ]_s = n - 1 /\ 1 <= n))%string.
+    intros s [xn x0].
+    apply cmd0.wp_assign_c.
+    rewrite state.eval_upd_same.
+    unfold state.eval.
+    fold ([ % "x"%string ]_ s).
+    rewrite xn.
+    unfold state.eval at 2 in x0.
+    omega.
+  apply C.hoare_basic.
+  now apply cmd0.hoare0_assign.
+(* call; x <- x + 1; ... *)
+apply C.hoare_seq with (fun s => [% "x" ]_s = n - 1 /\ [ % "ret" ]_ s = fact (n - 1) /\ 1 <= n)%string.
+(*  apply C.hoare_conseq_spec with (fun s => [ %"x" ]_s = n - 1)%string
+    (fun s => [ %"x" ]_s = n - 1 /\ [ % "ret" ]_ s = fact (n - 1))%string.
+  intros ? ?.
+  tauto.
+  intros s [xn1 Hfact].
+  intuition.
+  admit.
+  apply C.hoare_call2.
+  apply Union_intror.
+  assert (InSpecsn1 : In (BIGCUP X factospec) (factospec (n - 1))).
+    apply In_BIGCUP.
+    omega.
+  now unfold factospec at 2 in InSpecsn1.*)
+  apply C.hoare_conseq.
+  intros s [xn1 onen].
+  exists (fun s => [ % "x"%string ]_s = n - 1),
+    (fun s => [ % "x" ]_s = n - 1 /\ [ % "ret" ]_s = fact (n - 1))%string.
+  split.
+    apply C.hoare_call2.
+    apply Union_intror.
+    assert (InSpecsn1 : In (BIGCUP X factospec) (factospec (n - 1))).
+      apply In_BIGCUP.
+      omega.
+    now unfold factospec at 2 in InSpecsn1.
+  split; [now auto | ].
+  intros ? ?.
+  tauto.
+(* x <- x + 1; ret <- ret * x *)
+apply C.hoare_seq with (fun s => [% "x" ]_s = n /\ [ % "ret" ]_s = fact (n - 1) /\ 1 <= n)%string.
+  apply C.hoare_stren with (cmd0.wp_assign "x" (% "x" \+ 1)
+                         (fun s => [ % "x" ]_s = n /\ [ % "ret" ]_s = fact (n - 1) /\ 1 <= n))%string.
+    intros s [xn1 Hret].
+    apply cmd0.wp_assign_c.
+    rewrite state.eval_upd_same.
+    rewrite state.eval_upd_diff; [ | now auto].
+    unfold state.eval at 1.
+    fold ([ % "x"%string ]_s).
+    rewrite xn1.
+    omega.
+  apply C.hoare_basic.
+  now apply cmd0.hoare0_assign.
+(* ret <- ret * x *)
+apply C.hoare_stren with (cmd0.wp_assign "ret" (% "ret" \* % "x")
+  (fun s => [ % "x" ]_s = n /\ [ % "ret" ]_s = fact n))%string.
+  intros s [xn [Hret onen]].
+  apply cmd0.wp_assign_c.
+  rewrite state.eval_upd_same.
+  rewrite state.eval_upd_diff; [ | now auto].
+  unfold state.eval at 2.
+  fold ([ % "x"%string ]_s).
+  fold ([ % "ret"%string ]_s).
+  rewrite Hret, xn.
+  rewrite fact_fact; tauto.
+apply C.hoare_basic.
+now apply cmd0.hoare0_assign.
+Qed.
+
+End FactorialRec.
